examples/wysteria/sem.fst
@@ -1,5 +1,5 @@
 (*--build-config
-    options:--admit_fsi FStar.OrdSet --admit_fsi FStar.OrdMap --admit_fsi Prins --admit_fsi Ffibridge --__temp_no_proj;
+    options:--admit_fsi FStar.OrdSet --admit_fsi FStar.OrdMap --admit_fsi Prins --admit_fsi Ffibridge;
     other-files:ghost.fst listTot.fst ordset.fsi ordmap.fsi classical.fst prins.fsi ast.fst ffibridge.fsi
  --*)
 
